tau_defer_fundef: now 75% cheat-free

projection/payload_closureScript.sml
@@ -55,7 +55,12 @@ Definition written_var_names_endpoint_before_def:
      []
    else
      written_var_names_endpoint_before dn e1 ++ written_var_names_endpoint_before dn e2)
-∧ (written_var_names_endpoint_before dn (FCall dv vars) = vars)
+∧ (written_var_names_endpoint_before dn (FCall dv vars) =
+    if dn = dv then
+       vars
+    else
+       []
+   )
 End
 
 Definition compile_endpoint_def:
@@ -69,7 +74,7 @@ Definition compile_endpoint_def:
     (compile_endpoint ar (Letrec dn vars e1 e2) = Nil (* Source term should use fixpoint style *)) ∧
     (compile_endpoint ar (FCall dn vars) = Nil (* Source term should use fixpoint style *)) ∧
     (compile_endpoint ar (Fix dn e) =
-     let vars = nub'(written_var_names_endpoint_until e);
+     let vars = nub'(written_var_names_endpoint e);
          e' = compile_endpoint ((dn,vars)::ar) e
      in
        Letrec dn vars e' (FCall dn vars)
